More work in src/ByteStringFMap.v

src/ByteStringFMap.v
@@ -51,7 +51,22 @@ Record PS' := {
 }.
 
 Variable heap' : ComputationalADT.cRep (projT1 HeapImpl).
-Variable AbsR : Heap_AbsR heap heap'.
+Variable AbsR : Heap_AbsR (` heap) heap'.
+
+Lemma refine_pick_PS' : forall P a b c d,
+  refine {r_n0 : PS' | P (ps'Heap r_n0) /\
+                       a = ps'Buffer r_n0 /\
+                       b = ps'BufLen r_n0 /\
+                       c = ps'Offset r_n0 /\
+                       d = ps'Length r_n0}
+         (r_n' <- {r_n0 : N * M.t MemoryBlockC | P r_n0};
+          {r_n0 : PS' | r_n' = ps'Heap   r_n0 /\
+                        a = ps'Buffer r_n0 /\
+                        b = ps'BufLen r_n0 /\
+                        c = ps'Offset r_n0 /\
+                        d = ps'Length r_n0}).
+Proof.
+Admitted.
 
 (* Strip away the proofy bits. *)
 Lemma ByteStringStrip :
@@ -60,7 +75,7 @@ Proof.
   eexists.
   hone representation using
        (fun (or : PS) (nr : PS') =>
-          Heap_AbsR (psHeap or) (ps'Heap nr) /\
+          Heap_AbsR (` (psHeap or)) (ps'Heap nr) /\
           psBuffer or = ps'Buffer nr /\
           psBufLen or = ps'BufLen nr /\
           psOffset or = ps'Offset nr /\
@@ -76,69 +91,85 @@ Proof.
     simpl; intuition.
   }
   {
-    destruct (psHeap r_o); simpl in *.
     repeat match goal with
       [ H : _ /\ _ |- _ ] => destruct H
     end; subst.
     rewrite H1; clear H1.
     rewrite H2; clear H2.
     rewrite H3; clear H3.
+    rewrite H4; clear H4.
     rewrite refineEquiv_If_Then_Else_Bind.
     apply refine_If_Then_Else.
       simplify with monad laws; simpl.
-      unfold Heap_AbsR, poke', poke; simpl.
+      unfold poke'; simpl.
       remove_dependency; simpl.
-      simplify with monad laws; simpl.
-      {
+      etransitivity.
+        apply refine_under_bind; intros.
+        rewrite refine_pick_PS'.
+        simplify with monad laws.
+        finish honing.
+      simpl.
+      rewrite
+        (Heap_refine_poke
+           H0 _ _
+           (fun u =>
+              r_n' <- { r_n0 : PS' |
+                        fst u             = ps'Heap   r_n0 /\
+                        ps'Buffer r_n     = ps'Buffer r_n0 /\
+                        ps'BufLen r_n     = ps'BufLen r_n0 /\
+                        ps'Offset r_n - 1 = ps'Offset r_n0 /\
+                        ps'Length r_n + 1 = ps'Length r_n0 };
+              ret (r_n', ()))).
+        remember (M.mapi _ _) as M.
         refine pick val
-          {| ps'Heap :=
-               (fst (ps'Heap r_n),
-                M.mapi
-                  (fun (base : N) (blk : MemoryBlockC) =>
-                     IfDec (within base (memCSize blk)
-                                   (ps'Buffer r_n + (ps'Offset r_n - 1)))
-                     Then {| memCSize := memCSize blk
-                             ; memCData :=
-                                 M.add (ps'Buffer r_n + (ps'Offset r_n - 1)
-                                                        - base) d
-                                       (memCData blk) |}
-                     Else blk)
-                  (snd (ps'Heap r_n)))
+          {| ps'Heap   := (fst (ps'Heap r_n), M)
            ; ps'Buffer := ps'Buffer r_n
            ; ps'BufLen := ps'BufLen r_n
            ; ps'Offset := ps'Offset r_n - 1
            ; ps'Length := ps'Length r_n + 1 |}.
           simplify with monad laws.
+          rewrite HeqM.
           finish honing.
         simpl; intuition.
-        - apply FunMaps.Map_Map_AbsR; eauto.
-          + relational.
-          + relational.
-          + relational.
-            rewrite (proj1 H2).
-            decisions; auto.
-            apply MemoryBlock_AbsR_AbsR; auto.
-            apply FunMaps.Update_Map_AbsR; auto.
-            exact (proj2 H2).
-          + exact (proj1 H0).
-        - apply (@Poke_in_heap (exist _ x f)); auto.
-        - rewrite H4; reflexivity.
-      }
+      exact (proj2_sig (psHeap r_o)).
     rewrite refineEquiv_If_Then_Else_Bind.
     subst H.
-    replace (psLength r_o <? ps'BufLen r_n)
-       with (ps'Length r_n <? ps'BufLen r_n)
-         by (rewrite H4; reflexivity).
     apply refine_If_Then_Else.
       simplify with monad laws; simpl.
-      unfold Heap_AbsR, memcpy', poke', memcpy, FindBlockThatFits.
-      remove_dependency.
-      setoid_rewrite refine_bind_dep_bind_ret.
+      unfold memcpy', poke'; simpl.
+      remove_dependency; simpl.
+      setoid_rewrite refine_bind_dep_bind_ret; simpl.
+      do 2 setoid_rewrite refine_bind_dep_ignore.
+      setoid_rewrite refine_pick_PS'.
+      etransitivity.
+        apply refine_under_bind; intros.
+        etransitivity.
+          apply refine_under_bind; intros.
+          simplify with monad laws.
+          finish honing.
+        simpl.
+        finish honing.
+      simpl.
+      rewrite N.add_0_r.
+(*
+      rewrite
+        (Heap_refine_poke
+           _ _ _
+           (fun u =>
+              r_n' <- {r_n0 : PS' |
+                       fst u             = ps'Heap   r_n0 /\
+                       ps'Buffer r_n     = ps'Buffer r_n0 /\
+                       ps'BufLen r_n     = ps'BufLen r_n0 /\
+                       0                 = ps'Offset r_n0 /\
+                       ps'Length r_n + 1 = ps'Length r_n0};
+              ret (r_n', ()))).
+
+        rewrite Heap_refine_poke.
       setoid_rewrite refine_bind_dep_ret; simpl.
       remove_dependency.
       simplify with monad laws; simpl.
-      rewrite H4.
-      finish honing.
+*)
+      admit.
     rewrite refineEquiv_If_Then_Else_Bind.
     apply refine_If_Then_Else.
       simplify with monad laws; simpl.
@@ -147,9 +178,10 @@ Proof.
       do 3 setoid_rewrite refine_bind_dep_bind_ret.
       simpl; remove_dependency.
       do 3 setoid_rewrite refine_bind_dep_ignore.
-      rewrite H4.
       unfold ByteStringHeap.buffer_cons_obligation_2.
-      finish honing.
+      erewrite Heap_refine_alloc'; eauto.
+        admit.
+      exact (proj2_sig (psHeap r_o)).
     unfold allocate_buffer, alloc', poke'.
     simplify with monad laws; simpl.
     remove_dependency.
@@ -157,7 +189,7 @@ Proof.
     autorewrite with monad laws; simpl.
     remove_dependency.
     unfold ByteStringHeap.buffer_cons_obligation_3.
-    finish honing.
+    admit.
   }
   {
     repeat match goal with
@@ -171,7 +203,7 @@ Proof.
       unfold peek'.
       remove_dependency.
       destruct (psHeap r_o); simpl in *; subst.
-      finish honing.
+      admit.
     simplify with monad laws; simpl.
     refine pick val r_n.
       simplify with monad laws; simpl.
@@ -179,700 +211,8 @@ Proof.
     intuition.
   }
   apply reflexivityT.
-Defined.
-
-Record PS'' := {
-  ps''Heap : ;
-
-  ps''Buffer : N;
-  ps''BufLen : N;
-
-  ps''Offset : N;
-  ps''Length : N
-}.
-
-Lemma ByteStringImpl : FullySharpened (projT1 ByteStringStrip).
-Proof.
-  start sharpening ADT.
-  hone representation using
-       (fun (or : PS') (nr : PS'') =>
-          Heap_AbsR (ps'Heap or) (ps''Heap nr) /\
-          ps'Buffer or = ps''Buffer nr /\
-          ps'BufLen or = ps''BufLen nr /\
-          ps'Offset or = ps''Offset nr /\
-          ps'Length or = ps''Length nr);
-  try simplify with monad laws; simpl; subst.
-  {
-    refine pick eq.
-    finish honing.
-  }
-  {
-    rewrite refineEquiv_If_Then_Else_Bind.
-    apply refine_If_Then_Else.
-      refine pick eq.
-      simplify with monad laws; simpl.
-      unfold poke'.
-      remove_dependency.
-      unfold Adt.Heap.poke.
-      rewrite refine_bind_dep_ret; simpl.
-      finish honing.
-    rewrite refineEquiv_If_Then_Else_Bind.
-    subst H.
-    apply refine_If_Then_Else.
-      refine pick eq.
-      simplify with monad laws; simpl.
-      unfold memcpy', poke'.
-      remove_dependency.
-      setoid_rewrite refine_bind_dep_bind_ret.
-      unfold Adt.Heap.memcpy, Adt.Heap.poke,
-             Adt.Heap.FindBlockThatFits.
-      setoid_rewrite refine_bind_dep_ret; simpl.
-    refine pick eq.
-    autorewrite with monad laws.
-    unfold poke'.
-    remove_dependency.
-    unfold Adt.Heap.poke.
-    rewrite refine_bind_dep_ret; simpl.
-    finish honing.
-  }
-  {
-    refine pick eq.
-    subst.
-    finish honing.
-  }
-  finish_SharpeningADT_WithoutDelegation.
-Defined.
-  
-
-Module Import BS := ByteString 
-Module Import Adt := HeapADT 
-Import Heap.
-
-Open Scope N_scope.
-
-Definition HSpec := projT1 HeapSpecADT.
-
-Definition memcpy' (r : Rep HSpec) (addr : N) (addr2 : N) (len : N) :
-  Comp (Rep HSpec * unit) :=
-  Eval simpl in callMeth HSpec memcpyS r addr addr2 len.
-
-Definition alloc' (r : Rep HSpec) (len : N | 0 < len) :
-  Comp (Rep HSpec * N) :=
-  Eval simpl in callMeth HSpec allocS r len.
-
-Definition free' (r : Rep HSpec) (addr : N) : Comp (Rep HSpec * unit) :=
-  Eval simpl in callMeth HSpec freeS r addr.
-
-Definition peek' (r : Rep HSpec) (addr : N) :
-  Comp (Rep HSpec * Word8) :=
-  Eval simpl in callMeth HSpec peekS r addr.
-
-Definition poke' (r : Rep HSpec) (addr : N) (w : Word8) :
-  Comp (Rep HSpec * unit) :=
-  Eval simpl in callMeth HSpec pokeS r addr w.
-
-Record PS := makePS {
-  psHeap : Rep HSpec;
-
-  psBuffer : N;
-  psBufLen : N;
-
-  psOffset : N;
-  psLength : N
-}.
-
-Definition simply_widen_region (r : PS) : PS :=
-  {| psHeap   := psHeap r
-   ; psBuffer := psBuffer r
-   ; psBufLen := psBufLen r
-   ; psOffset := psOffset r - 1
-   ; psLength := psLength r + 1 |}.
-
-Program Definition make_room_by_shifting_up (r : PS) (n : N | 0 < n) :
-  (* jww (2016-09-01): We could maybe be smarter by shifting the block so it
-     sits mid-way within the buffer. *)
-  Comp PS :=
-  res <- memcpy' (psHeap r) (psBuffer r) (psBuffer r + n) (psLength r);
-  ret {| psHeap   := fst res
-       ; psBuffer := psBuffer r
-       ; psBufLen := psBufLen r
-       ; psOffset := 0
-       ; psLength := psLength r + n |}.
-
-Program Definition make_room_by_growing_buffer (r : PS) (n : N | 0 < n) :
-  Comp PS :=
-  (* jww (2016-06-28): We can make a trade-off here by allocating extra bytes
-     in anticipation of future calls to [buffer_cons]. *)
-  `(h, a) <- alloc' (psHeap r) (psLength r + n);
-  `(h, _) <- memcpy' h (psBuffer r) (a + n) (psLength r);
-  `(h, _) <- free' h (psBuffer r);
-  ret {| psHeap   := h
-       ; psBuffer := a
-       ; psBufLen := psLength r + n
-       ; psOffset := 0
-       ; psLength := psLength r + n |}.
-Obligation 1. nomega. Qed.
-
-Program Definition allocate_buffer (r : Rep HSpec) (len : N | 0 < len) :
-  Comp PS :=
-  `(h, a) <- alloc' r len;
-  ret {| psHeap   := h
-       ; psBuffer := a
-       ; psBufLen := len
-       ; psOffset := 0
-       ; psLength := len |}.
-
-Definition poke_at_offset (r : PS) (d : Word8) : Comp PS :=
-  res <- poke' (psHeap r) (psBuffer r + psOffset r) d;
-  ret {| psHeap   := fst res
-       ; psBuffer := psBuffer r
-       ; psBufLen := psBufLen r
-       ; psOffset := psOffset r
-       ; psLength := psLength r |}.
-
-(* This defines how much a buffer is grown by when more space is needed to
-   [cons] on a new element. *)
-Definition alloc_quantum := 1.
-Arguments alloc_quantum /.
-
-Program Definition buffer_cons (r : PS) (d : Word8) : Comp PS :=
-  ps <- If 0 <? psOffset r
-        Then ret (simply_widen_region r)
-        Else If psLength r <? psBufLen r
-        Then make_room_by_shifting_up r alloc_quantum
-        Else If 0 <? psBufLen r
-        Then make_room_by_growing_buffer r alloc_quantum
-        Else allocate_buffer (psHeap r) alloc_quantum;
-  poke_at_offset ps d.
-Obligation 1. nomega. Qed.
-Obligation 2. nomega. Qed.
-Obligation 3. nomega. Qed.
-
-Definition buffer_uncons (r : PS) : Comp (PS * option Word8) :=
-  If 0 <? psLength r
-  Then (
-    w <- peek' (psHeap r) (psBuffer r + psOffset r);
-    ret ({| psHeap   := psHeap r
-          ; psBuffer := psBuffer r
-          ; psBufLen := psBufLen r
-          ; psOffset := if psLength r =? 1
-                        then 0
-                        else psOffset r + 1
-          ; psLength := psLength r - 1 |}, Some (snd w)))
-  Else ret (r, None).
-
-Definition ByteString_list_AbsR (or : Rep ByteStringSpec) (nr : PS) :=
-  length or = N.to_nat (psLength nr) /\
-  IF psBufLen nr = 0
-  then psOffset nr = 0 /\ psLength nr = 0
-  else
-    fits (psBuffer nr) (psBufLen nr)
-         (psBuffer nr + psOffset nr) (psLength nr) /\
-    exists data,
-      Lookup (psBuffer nr) {| memSize := psBufLen nr; memData := data |}
-             (` (psHeap nr)) /\
-      (forall i x, i < psLength nr
-                     -> nth (N.to_nat i) or x = x
-                     -> Lookup (psOffset nr + i) x data).
-
-Ltac destruct_AbsR H :=
-  let H1 := fresh "H1" in
-  let H2 := fresh "H2" in
-  destruct H as [H1 H2];
-  let H3 := fresh "H3" in
-  let H4 := fresh "H4" in
-  let data := fresh "data" in
-  destruct H2 as [[H [H2 H3]]|[H [H2 [data [H3 H4]]]]];
-  [ rewrite ?H, ?H2 in * | ].
-
-Ltac construct_AbsR := split; try split; simpl; try nomega.
-
-Ltac competing_lookups R H A1 H0 A2 :=
-  let Heqe := fresh "Heqe" in
-  destruct (A1 =? A2) eqn:Heqe;
-    [ apply Neqb_ok in Heqe; subst;
-      pose proof (allocations_unique (proj2_sig R) _ _ H _ H0);
-      subst; try nomega
-    | apply N.eqb_neq in Heqe;
-      pose proof (allocations_no_overlap (proj2_sig R) _ H _ H0 Heqe);
-      try nomega ].
-
-Ltac resolve_contention :=
-  match goal with
-  | [ H : All _ ?R, H0 : Lookup ?A ?B ?R |- _ ] => destruct (H A B)
-  end.
-
-Lemma refine_local_memcpy heap addr size len data :
-  fromADT HeapSpec heap ->
-  (0 < len -> fits addr size (addr + 1) len) ->
-  Lookup addr {| memSize := size; memData := data |} heap ->
-  refine
-    (ret (If 0 <? len
-          Then Update addr
-            {| memSize := size
-             ; memData :=
-                 Union _ (KeepKeys (not ∘ within 1 len) data)
-                         (ShiftKeys 0 1 (KeepKeys (within 0 len)
-                                                  data)) |}
-            heap
-          Else heap, tt))
-    (memcpy heap addr (addr + 1) len).
-Proof.
-  unfold memcpy; intro HH; intros.
-  unfold IfDec_Then_Else; simpl.
-  intros ??.
-  destruct (0 <? len) eqn:Heqe; simpl;
-  destruct_computations;
-  [|repeat teardown; intuition];
-  assert (H9 : 0 < len) by nomega; intuition.
-  destruct x, x0;
-  try destruct p;
-  try destruct p0.
-  - destruct H1, H2.
-    competing_lookups (exist _ heap HH) H n H2 n0;
-    competing_lookups (exist _ heap HH) H0 addr H2 n0.
-    replace (n0 - n0) with 0 by nomega.
-    replace (n0 + 1 - n0) with 1 by nomega.
-    constructor.
-  - destruct H1.
-    competing_lookups (exist _ heap HH) H0 addr H n.
-    resolve_contention; auto.
-  - destruct H2.
-    competing_lookups (exist _ heap HH) H0 addr H n.
-    resolve_contention; auto; nomega.
-  - resolve_contention; auto.
-Qed.
-
-Lemma simply_within : forall n m A (P Q : A),
-  0 < m -> IfDec within n m n Then P Else Q = P.
-Proof. intros; decisions; auto; nomega. Qed.
-
-Corollary within_nothing : forall addr p, ~ within addr 0 p.
-Proof. nomega. Qed.
-
-Lemma KeepKeys_nothing : forall P m,
-  (forall a, ~ P a) -> KeepKeys P m = Empty.
-Proof.
-  intros.
-  apply Extensionality_Ensembles, Same_Same_set.
-  split; unfold KeepKeys; intros;
-  teardown; firstorder.
-Qed.
-
-Lemma KeepKeys_everything : forall (P : N -> Prop) m,
-  (forall a, P a) -> KeepKeys P m = m.
-Proof.
-  intros.
-  apply Extensionality_Ensembles, Same_Same_set.
-  split; unfold KeepKeys; intros;
-  teardown; firstorder.
-Qed.
-
-Lemma ShiftKeys_nothing : forall a b, ShiftKeys a b Empty = Empty.
-Proof.
-  intros.
-  apply Extensionality_Ensembles, Same_Same_set.
-  split; unfold ShiftKeys; intros;
-  teardown; firstorder.
-Qed.
-
-Lemma memcpy_Update_inv :
-  forall r r' base1 addr1 blk1 base2 addr2 blk2 len,
-    memcpy r addr1 addr2 len ↝ r'
-      -> fits base1 (memSize blk1) addr1 len
-      -> fits base2 (memSize blk2) addr2 len
-      -> fromADT HeapSpec r
-      -> Lookup base1 blk1 r
-      -> Lookup base2 blk2 r
-      -> Lookup base2
-           {| memSize := memSize blk2
-            ; memData :=
-                let off1 := addr1 - base1 in
-                let off2 := addr2 - base2 in
-                Union
-                  _ (KeepKeys (not ∘ within off2 len) (memData blk2))
-                    (ShiftKeys off1 off2
-                               (KeepKeys (within off1 len)
-                                         (memData blk1))) |} (fst r').
-Proof.
-  intros.
-  destruct (0 <? len) eqn:Heqe.
-  - destruct_computations; simpl.
-    unfold IfDec_Then_Else; simpl.
-    rewrite Heqe.
-    destruct x, x0;
-    try destruct p;
-    try destruct p0.
-    + assert (base1 = n /\ base2 = n0).
-        repeat teardown.
-        competing_lookups (exist _ r H2) H3 base1 H n.
-        competing_lookups (exist _ r H2) H4 base2 H5 n0.
-      repeat teardown; simpl in *; subst.
-      left; intuition.
-      competing_lookups (exist _ r H2) H n H3 n.
-      competing_lookups (exist _ r H2) H5 n0 H4 n0.
-    + resolve_contention; assumption.
-    + clear H4.
-      resolve_contention; assumption.
-    + resolve_contention; assumption.
-  - assert (len = 0) by nomega.
-    rewrite H5 in *; clear H5.
-    destruct_computations; simpl in *.
-    unfold IfDec_Then_Else; simpl.
-    rewrite (KeepKeys_nothing _ (memData blk1)),
-            ShiftKeys_nothing,
-            KeepKeys_everything.
-    + destruct blk2; simpl in *.
-      assert (Union (N * Word8) memData0 Empty = memData0).
-        apply Extensionality_Ensembles.
-        split; intros; intros ??.
-          destruct H6; trivial.
-          inv H6.
-        left; assumption.
-      rewrite H6.
-      repeat teardown; assumption.
-    + unfold not, compose; intros; nomega.
-    + nomega.
-Qed.
-
-Theorem buffer_cons_sound
-        (r_o : list Word8) (r_n : PS)
-        (AbsR : ByteString_list_AbsR r_o r_n) :
-  forall x r_n' (H : buffer_cons r_n x ↝ r_n'),
-    ByteString_list_AbsR (x :: r_o) r_n'.
-Proof.
-  unfold buffer_cons; intros.
-  apply refine_computes_to_ret in H.
-  rewrite refineEquiv_If_Then_Else_Bind in H.
-  apply refine_If_Then_Else_bool in H.
-  destruct (0 <? psOffset r_n) eqn:Heqe.
-    apply refine_computes_to_ret in H.
-    {
-      destruct_computations; simpl.
-      destruct_AbsR AbsR; construct_AbsR.
-      right; intuition; [abstract nomega|].
-      exists (Update (psOffset r_n - 1) x data).
-      split; intros; teardown.
-        destruct_computations; tsubst; teardown.
-        exists {| memSize := psBufLen r_n; memData := data |}; simpl.
-        decisions; intuition.
-          f_equal; f_equal; abstract nomega.
-        destruct H2; abstract nomega.
-      destruct i using N.peano_ind.
-        left; abstract nomega.
-      right; split; [abstract nomega|].
-      rewrite <- N.add_sub_swap; [|abstract nomega].
-      rewrite <- N.add_sub_assoc; [|abstract nomega].
-      apply H4; [abstract nomega|].
-      rewrite N2Nat.inj_sub.
-      replace (N.to_nat 1) with 1%nat; [|abstract nomega].
-      simpl; rewrite N2Nat.inj_succ in *; simpl.
-      rewrite Nat.sub_0_r; assumption.
-    }
-  assert (psOffset r_n = 0) by abstract nomega; clear Heqe.
-  rewrite refineEquiv_If_Then_Else_Bind in H.
-  apply refine_If_Then_Else_bool in H.
-  destruct (psLength r_n <? psBufLen r_n) eqn:Heqe2;
-  [| rewrite refineEquiv_If_Then_Else_Bind in H;
-     destruct (0 <? psBufLen r_n) eqn:Heqe3; simpl in H ];
-  apply refine_computes_to_ret in H; revert H;
-  unfold make_room_by_shifting_up, make_room_by_growing_buffer,
-         allocate_buffer, poke_at_offset;
-  autorewrite with monad laws; simpl;
-  rewrite ?N.add_0_r;
-  unfold memcpy', alloc', free', poke';
-  rewrite refine_bind_dep_bind_ret; simpl;
-  repeat setoid_rewrite refine_bind_dep_bind_ret; simpl.
-  - simpl; intros; destruct_computations;
-    destruct_AbsR AbsR; construct_AbsR;
-    (right; split; [abstract nomega|]; split; [abstract nomega|]).
-    eapply refine_local_memcpy in x1; eauto;
-    [|exact (proj2_sig (psHeap r_n))|];
-    destruct (0 <? psLength r_n) eqn:Heqe;
-    try abstract nomega; destruct x1, x3; simpl in *.
-      eexists.
-      split.
-        teardown.
-        exists
-          {| memSize := psBufLen r_n
-           ; memData :=
-               Union _ (KeepKeys (not ∘ within 1 (psLength r_n)) data)
-                       (ShiftKeys 0 1 (KeepKeys (within 0 (psLength r_n))
-                                                data)) |}.
-        split.
-          rewrite simply_within; nomega.
-        teardown.
-      intros; teardown.
-      destruct i using N.peano_ind.
-        left; abstract nomega.
-      right; split; [abstract nomega|]; clear IHi.
-      simpl; rewrite N2Nat.inj_succ in *; simpl.
-      rewrite H0 in H4; simpl in H4.
-      unfold KeepKeys, ShiftKeys; teardown.
-      destruct (within_dec 0 (N.succ (psLength r_n)) (N.succ i)).
-        right; teardown.
-        exists (i, x0); simpl.
-        split.
-          f_equal; abstract nomega.
-        assert (i < psLength r_n) by abstract nomega.
-        specialize (H4 _ _ H6 H5).
-        teardown; intuition.
-        abstract nomega.
-      left; teardown.
-      split.
-        apply H4; [abstract nomega|].
-        rewrite N2Nat.inj_succ, nth_overflow; trivial.
-        abstract nomega.
-      unfold not, compose; intros.
-      contradiction n.
-      abstract nomega.
-    eexists.
-    split.
-      teardown.
-      exists {| memSize := psBufLen r_n; memData := data |}.
-      split; auto.
-      rewrite simply_within; nomega.
-    intros; teardown.
-    destruct i using N.peano_ind.
-      left; abstract nomega.
-    right; split; [abstract nomega|].
-    rewrite H0 in H4; simpl in H4; apply H4; [abstract nomega|].
-    simpl; rewrite N2Nat.inj_succ in *; simpl.
-    destruct r_o; simpl in *; auto; abstract nomega.
-  - simpl; intros;
-    apply Bind_dep_inv in H;
-    destruct H as [? [x1 ?]];
-    assert (fromADT HeapSpec (fst x0))
-      by (eapply alloc_fromADT; eauto;
-          [ exact (proj2_sig (psHeap r_n))
-          | simpl; apply refine_computes_to_ret; apply x1 ]).
-    simpl; intros; destruct_computations;
-    destruct_AbsR AbsR; construct_AbsR;
-    (right; split; [abstract nomega|]; split; [abstract nomega|]).
-    rewrite H0, N.add_0_r in *; simpl in *; clear H0.
-    pose proof (@memcpy_Update_inv
-                  (fst x0) x2
-                  (psBuffer r_n) (psBuffer r_n)
-                  {| memSize := psBufLen r_n; memData := data |}
-                  (snd x0) (snd x0 + 1)
-                  {| memSize := psLength r_n + 1; memData := Empty |}
-                  (psLength r_n) x3 H2).
-    simpl in H.
-    unfold alloc, FindFreeBlock in x1.
-    unfold free in x5.
-    destruct_computations; simpl in *; intros.
-    pose proof (H6 _ _ H3); simpl in *.
-    destruct (psLength r_n =? 0) eqn:Heqe.
-      apply Neqb_ok in Heqe.
-      rewrite Heqe in *; clear Heqe; simpl.
-      exists (Update 0 x Empty);
-      split; repeat teardown; subst; simpl; try abstract nomega.
-    assert (0 <? psLength r_n = true) by abstract nomega.
-    eexists; split.
-      apply Lookup_Map.
-      eexists
-        {| memSize := psLength r_n + 1
-         ; memData :=
-             Union _ (KeepKeys (not ∘ within 1 (psLength r_n)) Empty)
-                     (ShiftKeys 0 1 (KeepKeys (within 0 (psLength r_n))
-                                              data)) |}.
-      rewrite simply_within; simpl; [|abstract nomega].
-      replace (x1 - x1) with 0 by abstract nomega.
-      split.
-        reflexivity.
-      apply Lookup_Remove; [|abstract nomega].
-      simpl in *.
-      revert H0.
-      replace (psBuffer r_n - psBuffer r_n) with 0 by abstract nomega.
-      replace (x1 + 1 - x1) with 1 by abstract nomega.
-      intro H0.
-      {
-        apply H0.
-        + abstract nomega.
-        + assumption.
-        + assert (psBuffer r_n <> x1) by abstract nomega.
-          teardown.
-        + teardown.
-      }
-    destruct i using N.peano_ind;
-    simpl in *; intros; subst; teardown.
-    right; split; [abstract nomega|].
-    unfold ShiftKeys, KeepKeys.
-    teardown; right.
-    teardown; exists (i, x2); split; simpl.
-      f_equal; abstract nomega.
-    teardown.
-    split; [|abstract nomega].
-    apply H4; [abstract nomega|].
-    rewrite N2Nat.inj_succ in *; simpl.
-    assumption.
-  - simpl; intros; destruct_computations;
-    destruct_AbsR AbsR; construct_AbsR;
-    (right; split; [abstract nomega|]; split; [abstract nomega|]).
-    unfold alloc, FindFreeBlock in x1.
-    destruct_computations; simpl in *.
-    rewrite H3, ?N.add_0_r in *; simpl.
-    repeat teardown; subst; simpl; try abstract nomega;
-    exists (Update 0 x Empty);
-    split; repeat teardown;
-    try exists {| memSize := 1; memData := Empty |};
-    try split; repeat teardown;
-    decisions; simpl; auto;
-    replace (x1 - x1) with 0 by abstract nomega; auto;
-    try abstract nomega; simpl; intros;
-    try (destruct i using N.peano_ind; simpl in *; subst;
-         [ teardown | abstract nomega ]).
-Qed.
-
-Theorem buffer_uncons_sound : forall r_o r_n a,
-  ByteString_list_AbsR r_o r_n
-    -> buffer_uncons r_n ↝ a
-    -> ByteString_list_AbsR (match r_o with
-                             | [] => r_o
-                             | _ :: xs => xs
-                             end) (fst a).
-Proof.
-  unfold buffer_uncons; intros.
-  apply refine_computes_to_ret in H0.
-  apply refine_If_Then_Else_bool in H0.
-  destruct (0 <? psLength r_n) eqn:Heqe.
-    revert H0.
-    unfold peek'.
-    rewrite refine_bind_dep_bind_ret; simpl.
-    rewrite refine_bind_dep_ignore.
-    unfold peek, FindBlockThatFits.
-    autorewrite with monad laws; simpl; intros.
-    apply refine_computes_to_ret in H0.
-    destruct_computations.
-    destruct_AbsR H; construct_AbsR;
-    destruct x; try destruct p; simpl in *;
-    destruct r_o; simpl in *;
-    try nomega; right;
-    split; try nomega; split;
-    destruct (psLength r_n =? 1) eqn:Heqe2;
-    try nomega;
-    try (eexists; split; [exact H4|]; nomega);
-    (eexists;
-     split; [exact H4|];
-     intros;
-     rewrite <- N.add_assoc;
-     apply H5;
-     [ apply N.lt_add_lt_sub_l
-     | rewrite N.add_1_l, N2Nat.inj_succ ];
-     trivial).
-  apply refine_computes_to_ret in H0.
-  destruct_computations.
-  destruct_AbsR H; construct_AbsR;
-  destruct r_o; simpl in *; auto; try nomega.
-  - left; intuition.
-  - right; intuition.
-    eexists; intuition.
-    exact H3.
-Qed.
-
-Theorem buffer_uncons_impl : forall r_o r_n a,
-  ByteString_list_AbsR r_o r_n
-    -> buffer_uncons r_n ↝ a
-    -> snd a = match r_o with
-               | [] => None
-               | x :: _ => Some x
-               end.
-Proof.
-  unfold buffer_uncons; intros.
-  apply refine_computes_to_ret in H0.
-  apply refine_If_Then_Else_bool in H0.
-  destruct (0 <? psLength r_n) eqn:Heqe.
-    revert H0.
-    unfold peek'.
-    rewrite refine_bind_dep_bind_ret; simpl.
-    rewrite refine_bind_dep_ignore.
-    unfold peek, FindBlockThatFits.
-    autorewrite with monad laws; simpl; intros.
-    apply refine_computes_to_ret in H0.
-    destruct_computations.
-    destruct_AbsR H; simpl;
-    destruct r_o; simpl in *; try nomega.
-    f_equal.
-    destruct x; tsubst; simpl in *.
-      destruct p.
-      specialize (H1 w _ _ eq_refl); simpl in *.
-      apply H1.
-      destruct H0.
-      competing_lookups (psHeap r_n) H4 (psBuffer r_n) H0 n.
-      simpl in *.
-      replace (psBuffer r_n + psOffset r_n - psBuffer r_n)
-         with (psOffset r_n + 0) by nomega.
-      apply H5; nomega.
-    resolve_contention; trivial; nomega.
-  apply refine_computes_to_ret in H0.
-  apply Return_inv in H0.
-  destruct a; tsubst; simpl in *.
-  destruct r_o; simpl in *;
-  destruct H, H0; auto.
-    destruct H0, H1.
-    rewrite H2 in H; simpl in H.
-    discriminate.
-  nomega.
-Qed.
-
-Section Refined.
-
-Variable heap : Rep HSpec.
-
-Lemma ByteStringHeap  : { adt : _ & refineADT ByteStringSpec adt }.
-Proof.
-  eexists.
-  hone representation using ByteString_list_AbsR.
-  {
-    simplify with monad laws.
-    refine pick val {| psHeap   := heap
-                     ; psBuffer := 0
-                     ; psBufLen := 0
-                     ; psOffset := 0
-                     ; psLength := 0 |}.
-      finish honing.
-    split; simpl; auto.
-    left; auto.
-  }
-  {
-    simplify with monad laws.
-    etransitivity.
-      eapply (refine_skip2 (dummy:=buffer_cons r_n d)).
-    etransitivity.
-      apply refine_under_bind; intros; simpl.
-      refine pick val a.
-        simplify with monad laws.
-        finish honing.
-      eapply buffer_cons_sound; eauto.
-    unfold buffer_cons, simply_widen_region,
-           make_room_by_shifting_up, make_room_by_growing_buffer.
-    simplify with monad laws; simpl.
-    finish honing.
-  }
-  {
-    simplify with monad laws.
-    etransitivity.
-      eapply (refine_skip2 (dummy:=buffer_uncons r_n)).
-    etransitivity.
-      apply refine_under_bind; intros; simpl.
-      pose proof H1.
-      eapply buffer_uncons_impl in H1; eauto.
-      rewrite fst_match_list, snd_match_list, <- H1.
-      refine pick val (fst a).
-        simplify with monad laws.
-        rewrite <- surjective_pairing.
-        finish honing.
-      eapply buffer_uncons_sound; eauto.
-    simplify with monad laws.
-    unfold buffer_uncons.
-    finish honing.
-  }
-  apply reflexivityT.
-Defined.
-
-Definition ByteStringHeap' := Eval simpl in projT1 ByteStringHeap.
-Print ByteStringHeap'.
+Admitted.
 
 End Refined.
 
-End ByteStringHeap.
+End ByteStringFMap.
