src/HeapFMap.v
@@ -9,6 +9,7 @@ Require Import
   ByteString.HeapADT
   ByteString.Within
   ByteString.DefineAbsR
+  ByteString.Same_set
   Coq.FSets.FMapFacts
   Coq.Structures.DecidableTypeEx.
 
@@ -23,9 +24,9 @@ Import Block.FunMaps.
 Require Import Fiat.ADT Fiat.ADTNotation.
 
 Definition Heap_AbsR
-           (or : { r : Rep HeapSpec | fromADT HeapSpec r})
+           (or : Rep HeapSpec)
            (nr : N * M.t MemoryBlockC) : Prop :=
-  Map_AbsR MemoryBlock_AbsR (` or) (snd nr) /\
+  Map_AbsR MemoryBlock_AbsR or (snd nr) /\
   P.for_all (within_allocated_mem (fst nr)) (snd nr).
 
 Theorem heaps_refine_to_maps : forall r : Rep HeapSpec, fromADT _ r ->
@@ -50,11 +51,31 @@ Ltac apply_for_all :=
     pose proof (proj1 (@P.for_all_iff _ P H3 m) H1 k e H2)
   end.
 
+Ltac related_maps' :=
+  repeat (
+    related_maps; auto with maps;
+    try match goal with
+      [ |- MemoryBlock_AbsR {| memSize := _;  memData := _ |}
+                            {| memCSize := _; memCData := _ |} ] =>
+      apply MemoryBlock_AbsR_impl; auto with maps
+    end).
+
+Ltac AbsR_prep :=
+  repeat
+    match goal with
+    | [ H : Heap_AbsR _ _ |- _ ] => unfold Heap_AbsR in H; simpl in H
+    | [ |- Heap_AbsR _ _ ] => unfold Heap_AbsR; simpl
+    | [ H : _ /\ _ |- _ ] => destruct H; simpl in H
+    | [ |- _ /\ _ ] => split
+    end; simpl; eauto; eauto with maps; related_maps'.
+
+Require Import Fiat.ADTRefinement Fiat.ADTRefinement.BuildADTRefinements.
+
 Lemma Heap_AbsR_outside_mem
       {r_o r_n} (AbsR : Heap_AbsR r_o r_n)
       (d : {len : N | 0 < len}) :
   All (fun addr' blk' =>
-         ~ overlaps addr' (memSize blk') (fst r_n) (` d)) (` r_o).
+         ~ overlaps addr' (memSize blk') (fst r_n) (` d)) r_o.
 Proof.
   intros addr blk H.
   apply AbsR in H; destruct H as [? [? ?]].
@@ -63,7 +84,101 @@ Proof.
   apply_for_all. nomega.
 Qed.
 
-Theorem Peek_in_heap {r_o r_n} (AbsR : Heap_AbsR r_o r_n) pos :
+Lemma refine_set_pair_same : forall A (x z : Comp A) B (y w : B),
+  Same_set _ x z -> y = w -> refine (ret (x, y)) (ret (z, w)).
+Proof.
+  intros; subst.
+  f_equiv.
+  f_equal.
+  apply Extensionality_Ensembles.
+  assumption.
+Qed.
+
+Theorem Heap_refine_alloc' `(AbsR : Heap_AbsR r_o r_n) d :
+ fromADT HeapSpec r_o ->
+  refine
+    (alloc r_o d)
+    (ret (of_map MemoryBlock_AbsR
+                 (M.add (fst r_n)
+                        {| memCSize := proj1_sig d
+                         ; memCData := M.empty _ |} (snd r_n)), fst r_n)).
+Proof.
+  intros.
+  unfold alloc, FindFreeBlock.
+  refine pick val (fst r_n).
+    simplify with monad laws; simpl.
+    apply refine_set_pair_same; auto.
+    apply Same_Same_set, of_map_Same.
+    destruct AbsR.
+    related_maps'.
+  apply Heap_AbsR_outside_mem; assumption.
+Qed.
+
+Theorem Heap_refine_alloc `(AbsR : Heap_AbsR r_o r_n) d :
+ fromADT HeapSpec r_o ->
+  refine
+    (x <- alloc r_o d;
+     r_n' <- {r_n0 : N * M.t MemoryBlockC | Heap_AbsR (fst x) r_n0};
+     ret (r_n', snd x))
+    (ret ((fst r_n + proj1_sig d,
+           M.add (fst r_n)
+                 {| memCSize := proj1_sig d
+                  ; memCData := M.empty _ |} (snd r_n)), fst r_n)).
+Proof.
+  intros.
+  remember (fst r_n + _, _) as r_n'.
+  unfold alloc, FindFreeBlock.
+  simplify with monad laws; simpl.
+  refine pick val (fst r_n).
+    simplify with monad laws; simpl.
+    refine pick val r_n'.
+      simplify with monad laws; simpl.
+      rewrite Heqr_n'.
+      reflexivity.
+    rewrite Heqr_n'.
+    destruct AbsR.
+    AbsR_prep.
+    apply for_all_add_iff; auto.
+      unfold not; intros.
+      apply (proj1 (in_mapsto_iff _ _ _)) in H2.
+      destruct H2.
+      apply_for_all.
+      apply H0 in H2; destruct H2, H2.
+      pose proof (allocations_have_size H _ _ H2).
+      rewrite (proj1 H5) in H6.
+      abstract nomega.
+    split.
+      apply for_all_impl
+       with (P':=within_allocated_mem (fst r_n + ` d)) in H1; auto.
+      abstract nomega.
+    abstract nomega.
+  apply Heap_AbsR_outside_mem; assumption.
+Qed.
+
+Theorem Heap_refine_free `(AbsR : Heap_AbsR r_o r_n) d :
+ fromADT HeapSpec r_o ->
+  refine
+    (x <- free r_o d;
+     r_n' <- {r_n0 : N * M.t MemoryBlockC | Heap_AbsR (fst x) r_n0};
+     ret (r_n', snd x))
+    (ret ((fst r_n, M.remove d (snd r_n)), tt)).
+Proof.
+  intros.
+  remember (fst r_n, _) as r_n'.
+  simplify with monad laws; simpl.
+  refine pick val r_n'.
+    simplify with monad laws.
+    rewrite Heqr_n'.
+    finish honing.
+  rewrite Heqr_n'.
+  destruct AbsR.
+  AbsR_prep.
+  apply for_all_remove; auto.
+Qed.
+
+Theorem Peek_in_heap
+        {r_o : { r | fromADT HeapSpec r }}
+        {r_n} (AbsR : Heap_AbsR (` r_o) r_n) pos :
   forall base blk' cblk',
     MemoryBlock_AbsR blk' cblk'
       -> Lookup base blk' (` r_o)
@@ -88,55 +203,240 @@ Proof.
   tauto.
 Qed.
 
-Theorem Poke_in_heap {r_o r_n} (AbsR : Heap_AbsR r_o r_n) pos val :
-  P.for_all (within_allocated_mem (fst r_n))
-    (M.mapi
-       (fun (addr : M.key) (cblk : MemoryBlockC) =>
-        IfDec within addr (memCSize cblk) pos
-        Then {| memCSize := memCSize cblk
-              ; memCData := M.add (pos - addr) val (memCData cblk) |}
-        Else cblk) (snd r_n)).
+Theorem Heap_refine_poke `(AbsR : Heap_AbsR r_o r_n) d d0
+        T (k : _ -> Comp T) :
+ fromADT HeapSpec r_o ->
+  refine
+    (a <- poke r_o d d0;
+     r_n' <- {r_n0 : N * M.t MemoryBlockC | Heap_AbsR (fst a) r_n0 };
+     k (r_n', snd a))
+    (k ((fst r_n,
+         M.mapi (fun addr cblk =>
+                   IfDec within addr (memCSize cblk) d
+                   Then {| memCSize := memCSize cblk
+                         ; memCData := M.add (d - addr) d0
+                                             (memCData cblk) |}
+                   Else cblk) (snd r_n)), tt)).
 Proof.
-  destruct AbsR as [_ H].
+  intros.
+  remember (fst r_n, _) as r_n'.
+  simplify with monad laws; simpl.
+  refine pick val r_n'.
+    simplify with monad laws.
+    rewrite Heqr_n'.
+    finish honing.
+  rewrite Heqr_n'.
+  destruct AbsR.
+  AbsR_prep; relational.
+    swap_sizes; decisions; auto.
+    destruct H3.
+    related_maps'.
   unfold P.for_all.
   apply P.fold_rec_bis; auto; intros.
-  apply F.mapi_mapsto_iff in H0.
-  destruct H0, H0.
+  apply F.mapi_mapsto_iff in H2.
+  destruct H2, H2.
   simpl; intros; subst; auto.
   unfold within_allocated_mem, IfDec_Then_Else; simpl.
-  eapply P.for_all_iff in H; eauto.
-    unfold within_allocated_mem in H.
+  eapply P.for_all_iff in H1; eauto.
+    unfold within_allocated_mem in H1.
     decisions; simpl in *; auto;
     congruence; auto.
   intros; subst; reflexivity.
 Qed.
 
-Ltac related_maps' :=
-  repeat (
-    related_maps; auto with maps;
-    try match goal with
-      [ |- MemoryBlock_AbsR {| memSize := _;  memData := _ |}
-                            {| memCSize := _; memCData := _ |} ] =>
-      apply MemoryBlock_AbsR_impl; auto with maps
-    end).
+Theorem Heap_refine_memcpy `(AbsR : Heap_AbsR r_o r_n) d d0 d1 :
+ fromADT HeapSpec r_o ->
+  refine
+    (x0 <- memcpy r_o d d0 d1;
+     r_n' <- {r_n0 : N * M.t MemoryBlockC | Heap_AbsR (fst x0) r_n0};
+     ret (r_n', snd x0))
+    (ret ((if 0 <? d1
+           then
+             match (find_if (withinMemBlockC d) (snd r_n),
+                    find_if (withinMemBlockC d0) (snd r_n)) with
+             | (Some (saddr, src), Some (daddr, dst)) =>
+               if (Decidable_witness (P:=fits saddr (memCSize src) d  d1) &&
+                   Decidable_witness (P:=fits daddr (memCSize dst) d0 d1))%bool
+               then
+                 (fst r_n,
+                  M.add daddr
+                        {| memCSize := memCSize dst
+                           ; memCData :=
+                               let soff := d - saddr in
+                               let doff := d0 - daddr in
+                               let s := keep_keys (within_bool soff d1)
+                                                  (memCData src) in
+                               let d := keep_keys (negb ∘ within_bool doff d1)
+                                                  (memCData dst) in
+                               P.update d (shift_keys soff doff s)
 
-Ltac AbsR_prep :=
-  repeat
-    match goal with
-    | [ H : Heap_AbsR _ _ |- _ ] => unfold Heap_AbsR in H; simpl in H
-    | [ |- Heap_AbsR _ _ ] => unfold Heap_AbsR; simpl
-    | [ H : _ /\ _ |- _ ] => destruct H; simpl in H
-    | [ |- _ /\ _ ] => split
-    end; simpl; eauto; eauto with maps; related_maps'.
+                        (* jww (2016-08-11): This version is more efficient in
+                        a strictly evaluated environment, but I'm having
+                        difficulty proving correspondence of the folds. *)
 
-Require Import Fiat.ADTRefinement Fiat.ADTRefinement.BuildADTRefinements.
+                        (* let soff := d - saddr in *)
+                        (* let doff := d0 - daddr in *)
+                        (* M.fold (fun k e m => *)
+                        (*           if within_bool soff d1 k *)
+                        (*           then M.add (k - soff + doff) e m *)
+                        (*           else m) (memCData src) *)
+                        (*        (keep_keys (negb ∘ within_bool doff d1) *)
+                        (*                   (memCData dst)) *)
+                        |}
+                        (snd r_n))
+               else r_n
+             | _ => r_n
+             end
+           else r_n), tt)).
+Proof.
+  intros.
+  remember (if 0 <? d1 then _ else _) as r_n'.
+  unfold memcpy, FindBlockThatFits.
+  simplify with monad laws; simpl.
+
+  refine pick val
+    (Ifopt find_if (withinMemBlockC d) (snd r_n) as p
+     Then if Decidable_witness (P:=fits (fst p) (memCSize (snd p)) d d1)
+          then Some (fst p,
+                     {| memSize := memCSize (snd p)
+                      ; memData := of_map eq (memCData (snd p)) |})
+          else None
+     Else None).
+    Focus 2.
+    destruct (find_if _ (snd r_n)) eqn:Heqe1; simpl in *.
+    destruct ((fst p <=? d)
+                && (d <? fst p + memCSize (snd p))
+                && (d + d1 <=? fst p + memCSize (snd p))) eqn:Heqe.
+        split; [|nomega].
+        apply find_if_inv in Heqe1; auto.
+        apply AbsR; exists (snd p); intuition.
+      apply find_if_inv in Heqe1; auto.
+      unfold withinMemBlockC in Heqe1;
+      simpl in Heqe1; destruct Heqe1.
+      apply andb_false_iff in Heqe; destruct Heqe.
+        congruence.
+      apply AbsR in H0; destruct H0 as [blk [? ?]].
+      intros ????.
+      destruct (fst p =? a) eqn:Heqe2.
+        apply Neqb_ok in Heqe2; subst.
+        pose proof (allocations_unique H _ _ H0 _ H4); subst.
+        rewrite (proj1 H3) in H5.
+        nomega.
+      apply N.eqb_neq in Heqe2.
+      apply within_reflect in H1.
+      rewrite <- (proj1 H3) in H1.
+      pose proof (allocations_disjoint H _ H0 H1 _ H4 Heqe2).
+      nomega.
+    apply find_if_not_inv in Heqe1; auto.
+    assert (Proper (eq ==> eq ==> eq) (negb \oo withinMemBlockC d)) by auto.
+    intros ????.
+    apply AbsR in H1; destruct H1 as [cblk [? ?]].
+    pose proof (proj1 (P.for_all_iff H0 _) Heqe1 _ _ H1).
+    unfold withinMemBlockC in H4; simpl in H4.
+    rewrite (proj1 H3) in H2.
+    unfold negb in H4.
+    destruct ((a <=? d) && (d <? a + memCSize cblk)) eqn:Heqe.
+      discriminate.
+    nomega.
+
+  simplify with monad laws.
+  refine pick val
+    (Ifopt find_if (withinMemBlockC d0) (snd r_n) as p
+     Then if Decidable_witness (P:=fits (fst p) (memCSize (snd p)) d0 d1)
+          then Some (fst p,
+                     {| memSize := memCSize (snd p)
+                      ; memData := of_map eq (memCData (snd p)) |})
+          else None
+     Else None).
+    Focus 2.
+    destruct (find_if (withinMemBlockC d0) (snd r_n)) eqn:Heqe1; simpl in *.
+    destruct ((fst p <=? d0)
+                && (d0 <? fst p + memCSize (snd p))
+                && (d0 + d1 <=? fst p + memCSize (snd p))) eqn:Heqe.
+        split; [|nomega].
+        apply find_if_inv in Heqe1; auto.
+        apply AbsR; exists (snd p); intuition.
+      apply find_if_inv in Heqe1; auto.
+      unfold withinMemBlockC in Heqe1;
+      simpl in Heqe1; destruct Heqe1.
+      apply andb_false_iff in Heqe; destruct Heqe.
+        congruence.
+      apply AbsR in H0; destruct H0 as [blk [? ?]].
+      intros ????.
+      destruct (fst p =? a) eqn:Heqe2.
+        apply Neqb_ok in Heqe2; subst.
+        pose proof (allocations_unique H _ _ H0 _ H4); subst.
+        rewrite (proj1 H3) in H5.
+        nomega.
+      apply N.eqb_neq in Heqe2.
+      apply within_reflect in H1.
+      rewrite <- (proj1 H3) in H1.
+      pose proof (allocations_disjoint H _ H0 H1 _ H4 Heqe2).
+      nomega.
+    apply find_if_not_inv in Heqe1; auto.
+    assert (Proper (eq ==> eq ==> eq) (negb \oo withinMemBlockC d0)) by auto.
+    intros ????.
+    apply AbsR in H1; destruct H1 as [cblk [? ?]].
+    pose proof (proj1 (P.for_all_iff H0 _) Heqe1 _ _ H1).
+    unfold withinMemBlockC in H4; simpl in H4.
+    rewrite (proj1 H3) in H2.
+    unfold negb in H4.
+    destruct ((a <=? d0) && (d0 <? a + memCSize cblk)) eqn:Heqe.
+      discriminate.
+    nomega.
+
+  simplify with monad laws; simpl.
+  refine pick val r_n'.
+    simplify with monad laws.
+    rewrite Heqr_n'.
+    finish honing.
+  rewrite Heqr_n'.
+  destruct AbsR.
+  AbsR_prep; clear H;
+  decisions; auto;
+  destruct (find_if (withinMemBlockC d) (snd r_n)) eqn:Heqe1;
+  try (apply find_if_inv in Heqe1; auto; destruct Heqe1);
+  destruct (find_if (withinMemBlockC d0) (snd r_n)) eqn:Heqe2;
+  try (apply find_if_inv in Heqe2; auto; destruct Heqe2);
+  simpl; auto; decisions;
+  try destruct p;
+  try destruct p0; simpl in *;
+  decisions; simpl; auto;
+  related_maps'; try nomega.
+  - apply Union_Map_AbsR; auto.
+    * apply KeepKeys_Map_AbsR.
+        apply not_within_AbsR.
+      apply of_map_Map_AbsR; auto.
+    * apply ShiftKeys_Map_AbsR.
+        constructor; apply KeepKeys_Map_AbsR.
+          apply within_AbsR; try reflexivity.
+        apply of_map_Map_AbsR; auto.
+      unfold KeepKeys; intros ???.
+      repeat teardown.
+      apply of_map_MapsTo in H6.
+      repeat teardown; subst; nomega.
+    * unfold not, compose, KeepKeys, ShiftKeys; intros ????.
+      repeat teardown; inv H6.
+      apply not_within_reflect in H5; nomega.
+  - discriminate.
+  - discriminate.
+  - rewrite <- remove_add.
+    apply for_all_add_true; auto.
+      simplify_maps.
+    split; trivial.
+      apply for_all_remove; auto.
+    simpl in *.
+    clear H2.
+    apply_for_all.
+    nomega.
+Qed.
 
 Lemma HeapImpl : FullySharpened HeapSpec.
 Proof.
   start sharpening ADT.
   eapply SharpenStep; [ apply (projT2 HeapSpecADT) |].
 
-  hone representation using Heap_AbsR.
+  hone representation using (fun or nr => Heap_AbsR (` or) nr).
 
   refine method emptyS.
   {
@@ -153,51 +453,16 @@ Proof.
 
   refine method allocS.
   {
-    unfold Heap_AbsR, alloc, FindFreeBlock.
     remove_dependency.
-    simplify with monad laws; simpl.
-
-    refine pick val (fst r_n).
-      Focus 2.
-      apply Heap_AbsR_outside_mem; trivial.
-
-    simplify with monad laws; simpl.
-    refine pick val (fst r_n + proj1_sig d,
-                     M.add (fst r_n)
-                           {| memCSize := proj1_sig d
-                            ; memCData := M.empty _ |} (snd r_n)).
-      simplify with monad laws.
-      finish honing.
-
-    AbsR_prep.
-    - apply for_all_add_iff; auto.
-      + unfold not; intros.
-        apply (proj1 (in_mapsto_iff _ _ _)) in H2.
-        destruct H2.
-        apply_for_all.
-        apply H0 in H2; destruct H2, H2.
-        pose proof (allocations_have_size (proj2_sig r_o) _ _ H2).
-        rewrite (proj1 H5) in H6.
-        abstract nomega.
-      + split.
-          apply for_all_impl
-           with (P':=within_allocated_mem (fst r_n + ` d)) in H1; auto.
-          abstract nomega.
-        abstract nomega.
+    destruct r_o.
+    eapply Heap_refine_alloc; eauto.
   }
 
   refine method freeS.
   {
-    unfold free.
     remove_dependency.
-    simplify with monad laws; simpl.
-
-    refine pick val (fst r_n, M.remove d (snd r_n)).
-      simplify with monad laws.
-      finish honing.
-
-    AbsR_prep.
-    - apply for_all_remove; auto.
+    destruct r_o.
+    eapply Heap_refine_free; eauto.
   }
 
   refine method reallocS.
@@ -371,196 +636,17 @@ Proof.
 
   refine method pokeS.
   {
-    unfold poke.
     remove_dependency.
-    simplify with monad laws; simpl.
-
-    refine pick val
-      (fst r_n,
-       M.mapi (fun addr cblk =>
-                 IfDec within addr (memCSize cblk) d
-                 Then {| memCSize := memCSize cblk
-                       ; memCData := M.add (d - addr) d0 (memCData cblk) |}
-                 Else cblk) (snd r_n)).
-      simplify with monad laws.
-      finish honing.
-
-    pose proof (Poke_in_heap H0).
-    AbsR_prep; relational; clear H.
-    - swap_sizes; decisions; auto.
-      related_maps'; exact (proj2 H4).
+    destruct r_o.
+    erewrite Heap_refine_poke; eauto.
+    finish honing.
   }
 
   refine method memcpyS.
   {
-    unfold Heap_AbsR, memcpy, FindBlockThatFits.
     remove_dependency.
-    simplify with monad laws; simpl.
-
-    refine pick val
-      (Ifopt find_if (withinMemBlockC d) (snd r_n) as p
-       Then if Decidable_witness (P:=fits (fst p) (memCSize (snd p)) d d1)
-            then Some (fst p,
-                       {| memSize := memCSize (snd p)
-                        ; memData := of_map eq (memCData (snd p)) |})
-            else None
-       Else None).
-      Focus 2.
-      destruct (find_if _ (snd r_n)) eqn:Heqe1; simpl in *;
-      decisions; simpl.
-          split; [|nomega].
-          apply find_if_inv in Heqe1; auto.
-          apply H0; exists (snd p); intuition.
-        apply find_if_inv in Heqe1; auto.
-        unfold withinMemBlockC in Heqe1;
-        simpl in Heqe1; destruct Heqe1.
-        apply andb_false_iff in Heqe; destruct Heqe.
-          congruence.
-        apply H0 in H1; destruct H1 as [blk [? ?]].
-        intros ????.
-        destruct (fst p =? a) eqn:Heqe.
-          apply Neqb_ok in Heqe; subst.
-          pose proof (allocations_unique (proj2_sig r_o) _ _ H1 _ H5); subst.
-          rewrite (proj1 H4) in H6.
-          nomega.
-        apply N.eqb_neq in Heqe.
-        apply within_reflect in H2.
-        rewrite <- (proj1 H4) in H2.
-        pose proof (allocations_disjoint (proj2_sig r_o)
-                                         _ H1 H2 _ H5 Heqe).
-        nomega.
-      apply find_if_not_inv in Heqe1; auto.
-      assert (Proper (eq ==> eq ==> eq) (negb \oo withinMemBlockC d)) by auto.
-      intros ????.
-      apply H0 in H2; destruct H2 as [cblk [? ?]].
-      pose proof (proj1 (P.for_all_iff H1 _) Heqe1 _ _ H2).
-      unfold withinMemBlockC in H5; simpl in H5.
-      rewrite (proj1 H4) in H3.
-      unfold negb in H5.
-      decisions; [discriminate|nomega].
-
-    simplify with monad laws.
-    refine pick val
-      (Ifopt find_if (withinMemBlockC d0) (snd r_n) as p
-       Then if Decidable_witness (P:=fits (fst p) (memCSize (snd p)) d0 d1)
-            then Some (fst p,
-                       {| memSize := memCSize (snd p)
-                        ; memData := of_map eq (memCData (snd p)) |})
-            else None
-       Else None).
-      Focus 2.
-      destruct (find_if _ (snd r_n)) eqn:Heqe1; simpl in *;
-      decisions; simpl.
-          split; [|nomega].
-          apply find_if_inv in Heqe1; auto.
-          apply H0; exists (snd p); intuition.
-        apply find_if_inv in Heqe1; auto.
-        unfold withinMemBlockC in Heqe1;
-        simpl in Heqe1; destruct Heqe1.
-        apply andb_false_iff in Heqe; destruct Heqe.
-          congruence.
-        apply H0 in H1; destruct H1 as [blk [? ?]].
-        intros ????.
-        destruct (fst p =? a) eqn:Heqe.
-          apply Neqb_ok in Heqe; subst.
-          pose proof (allocations_unique (proj2_sig r_o) _ _ H1 _ H5); subst.
-          rewrite (proj1 H4) in H6.
-          nomega.
-        apply N.eqb_neq in Heqe.
-        apply within_reflect in H2.
-        rewrite <- (proj1 H4) in H2.
-        pose proof (allocations_disjoint (proj2_sig r_o)
-                                         _ H1 H2 _ H5 Heqe).
-        nomega.
-      apply find_if_not_inv in Heqe1; auto.
-      assert (Proper (eq ==> eq ==> eq) (negb \oo withinMemBlockC d0)) by auto.
-      intros ????.
-      apply H0 in H2; destruct H2 as [cblk [? ?]].
-      pose proof (proj1 (P.for_all_iff H1 _) Heqe1 _ _ H2).
-      unfold withinMemBlockC in H5; simpl in H5.
-      rewrite (proj1 H4) in H3.
-      unfold negb in H5.
-      decisions; [discriminate|nomega].
-
-    simplify with monad laws.
-    refine pick val
-      (if 0 <? d1
-       then
-         match (find_if (withinMemBlockC d) (snd r_n),
-                find_if (withinMemBlockC d0) (snd r_n)) with
-         | (Some (saddr, src), Some (daddr, dst)) =>
-           if (Decidable_witness (P:=fits saddr (memCSize src) d  d1) &&
-               Decidable_witness (P:=fits daddr (memCSize dst) d0 d1))%bool
-           then
-             (fst r_n,
-              M.add daddr
-                {| memCSize := memCSize dst
-                 ; memCData :=
-                     let soff := d - saddr in
-                     let doff := d0 - daddr in
-                     let s := keep_keys (within_bool soff d1) (memCData src) in
-                     let d := keep_keys (negb ∘ within_bool doff d1)
-                                        (memCData dst) in
-                     P.update d (shift_keys soff doff s)
-
-                     (* jww (2016-08-11): This version is more efficient in a
-                        strictly evaluated environment, but I'm having
-                        difficulty proving correspondence of the folds. *)
-
-                     (* let soff := d - saddr in *)
-                     (* let doff := d0 - daddr in *)
-                     (* M.fold (fun k e m => *)
-                     (*           if within_bool soff d1 k *)
-                     (*           then M.add (k - soff + doff) e m *)
-                     (*           else m) (memCData src) *)
-                     (*        (keep_keys (negb ∘ within_bool doff d1) *)
-                     (*                   (memCData dst)) *)
-                 |}
-                (snd r_n))
-           else r_n
-         | _ => r_n
-         end
-       else r_n).
-      simplify with monad laws.
-      finish honing.
-
-    AbsR_prep; clear H;
-    decisions; auto;
-    destruct (find_if (withinMemBlockC d) (snd r_n)) eqn:Heqe1;
-    try (apply find_if_inv in Heqe1; auto; destruct Heqe1);
-    destruct (find_if (withinMemBlockC d0) (snd r_n)) eqn:Heqe2;
-    try (apply find_if_inv in Heqe2; auto; destruct Heqe2);
-    simpl; auto; decisions;
-    try destruct p;
-    try destruct p0; simpl in *;
-    decisions; simpl; auto;
-    related_maps'; try nomega.
-    - apply Union_Map_AbsR; auto.
-      * apply KeepKeys_Map_AbsR.
-          apply not_within_AbsR.
-        apply of_map_Map_AbsR; auto.
-      * apply ShiftKeys_Map_AbsR.
-          constructor; apply KeepKeys_Map_AbsR.
-            apply within_AbsR; try reflexivity.
-          apply of_map_Map_AbsR; auto.
-        unfold KeepKeys; intros ???.
-        repeat teardown.
-        apply of_map_MapsTo in H6.
-        repeat teardown; subst; nomega.
-      * unfold not, compose, KeepKeys, ShiftKeys; intros ????.
-        repeat teardown; inv H6.
-        apply not_within_reflect in H5; nomega.
-    - discriminate.
-    - discriminate.
-    - rewrite <- remove_add.
-      apply for_all_add_true; auto.
-        simplify_maps.
-      split; trivial.
-        apply for_all_remove; auto.
-      simpl in *.
-      clear H2.
-      apply_for_all.
-      nomega.
+    destruct r_o.
+    eapply Heap_refine_memcpy; eauto.
   }
 
   refine method memsetS.
